examples/store/proofs/base.v
@@ -80,7 +80,7 @@ Definition db_disconnected skI skR : iProp := ∃ db,
   DB.db_state skI skR dbN db.
 
 Definition db_connected' skI skR cs : iProp := ∃ db,
-  (compromised Init cs ∨ db_client_ready skI skR db) ∗
+  (compromised cs ∨ db_client_ready skI skR db) ∗
   DB.db_state skI skR dbN db.
 
 Definition db_connected skI skR cs : iProp :=
@@ -91,12 +91,20 @@ Lemma db_connected_ok skI skR cs :
   db_connected skI skR cs -∗
   secret skI -∗
   secret skR -∗
-  minted skI -∗
-  minted skR -∗
-  ◇ □ ¬ compromised Init cs.
+  ◇ session_ok cs.
 Proof.
 iIntros "(conn & _)".
 iApply (RPC.client_connected_ok with "conn").
+Qed.
+
+Lemma db_connected_ok_compromised skI skR cs :
+  db_connected skI skR cs -∗
+  session_ok cs -∗
+  compromised cs -∗
+  ▷ False.
+Proof.
+iIntros "(conn & _)".
+by iApply RPC.client_connected_ok_compromise.
 Qed.
 
 Definition db_mapsto skI skR t1 t2 : iProp :=
@@ -147,7 +155,7 @@ Qed.
 Definition server_db_connected' skI skR cs vdb : iProp := ∃ db,
   public_db db ∗
   AList.is_alist vdb (repr <$> db) ∗
-  (compromised Resp cs ∨ db_server_ready skI skR db).
+  (compromised cs ∨ db_server_ready skI skR db).
 
 Definition server_db_connected skI skR cs vdb : iProp :=
   RPC.server_connected skI skR cs ∗
@@ -204,7 +212,7 @@ Definition store_resp_pred skI skR si t t' : iProp :=
   ∃ db, rep_current skI skR dbN ∅ db.
 
 Lemma store_call t2' skI skR cs t1 t2 :
-  let P := compromised Init cs in
+  let P := compromised cs in
   db_connected' skI skR cs -∗
   db_mapsto skI skR t1 t2 ==∗
   (P ∨ store_call_pred skI skR cs (Spec.of_list [t1; t2'])) ∗
@@ -230,7 +238,7 @@ iExists _. iFrame. iRight. iFrame.
 Qed.
 
 Lemma store_resp skI skR cs db t1 t2 :
-  let P := compromised Resp cs in
+  let P := compromised cs in
   (P ∨ db_server_ready skI skR db) -∗
   (P ∨ store_call_pred skI skR cs (Spec.of_list [t1; t2])) ==∗
   (P ∨ db_server_ready skI skR (<[t1 := t2]>db)) ∗
@@ -251,7 +259,7 @@ Definition create_resp_pred skI skR si t t' : iProp :=
   ∃ db, rep_current skI skR dbN ∅ db.
 
 Lemma create_call t1 t2 skI skR cs :
-  let P := compromised Init cs in
+  let P := compromised cs in
   db_connected' skI skR cs -∗
   db_free_at skI skR {[t1]} ==∗
   (P ∨ create_call_pred skI skR cs (Spec.of_list [t1; t2])) ∗
@@ -276,7 +284,7 @@ iExists _. iFrame. iRight. iFrame.
 Qed.
 
 Lemma create_resp skI skR cs db t1 t2 :
-  let P := compromised Resp cs in
+  let P := compromised cs in
   (P ∨ db_server_ready skI skR db) -∗
   (P ∨ create_call_pred skI skR cs (Spec.of_list [t1; t2])) ==∗
   (P ∨ db_server_ready skI skR (<[t1 := t2]>db)) ∗
@@ -297,7 +305,7 @@ Definition load_resp_pred skI skR si t1 t2 : iProp :=
   ∃ db, ⌜db !! t1 = Some t2⌝ ∗ rep_current skI skR dbN ∅ db.
 
 Lemma load_call t1 t2 skI skR cs :
-  let P := compromised Init cs in
+  let P := compromised cs in
   db_connected' skI skR cs -∗
   db_mapsto skI skR t1 t2 ==∗
   (P ∨ load_call_pred skI skR cs t1) ∗
@@ -323,7 +331,7 @@ iSplit; eauto. iExists _. iFrame. iRight. iFrame.
 Qed.
 
 Lemma load_resp skI skR cs db t1 :
-  let P := compromised Resp cs in
+  let P := compromised cs in
   let t2 := default (TInt 0) (db !! t1) in
   (P ∨ db_server_ready skI skR db) -∗
   (P ∨ load_call_pred skI skR cs t1) ==∗
